Progress on HashThenSign.ec

proofs/Cleanup/HashThenSign.ec
@@ -5,10 +5,15 @@ require (*--*) Word Subtype ROM.
 (*---*) import RField IntOrder RealOrder BS2Int.
 
 (* -- Local -- *)
-require import Reprogramming.
-require (*--*) DigitalSignatures.
+require (*--*) DigitalSignatures Reprogramming EFRMA_Interactive_Equiv.
 
 
+
+(* Signature queries *)
+op qS : { int | 0 <= qS } as ge0_qS.
+
+(* Random oracle (hash) queries *)
+op qH : { int | 0 <= qH } as ge0_qH.  
 
 
 
@@ -49,7 +54,6 @@ clone import FinProdType as RCOMSGAL with
   theory FT1 <= RCO,
   theory FT2 <= MSG_AL.
 
-print RCOMSGAL.
 
 (* --- Distributions --- *)
 op [lossless] dmsg_fl : msg_fl_t distr.
@@ -61,24 +65,28 @@ op [lossless] drco : rco_t distr.
 
 
 (* --- Clones --- *)
-clone import DigitalSignatures as DSS1 with
-  type pk_t <- pk_fl_t,
-  type sk_t <- sk_fl_t,
-  type msg_t <- msg_fl_t,
-  type sig_t <- sig_fl_t
+clone import DigitalSignatures as DSS_FL with
+  type pk_t <= pk_fl_t,
+  type sk_t <= sk_fl_t,
+  type msg_t <= msg_fl_t,
+  type sig_t <= sig_fl_t.
   
-  rename [theory] "Stateless" as "FL_SL"
-  rename [theory] "KeyUpdating" as "FL_KU".
+clone import DigitalSignatures as DSS_AL with
+  type pk_t <= pk_al_t,
+  type sk_t <= sk_al_t,
+  type msg_t <= msg_al_t,
+  type sig_t <= sig_al_t.
 
-clone import DigitalSignatures as DSS2 with
-  type pk_t <- pk_al_t,
-  type sk_t <- sk_al_t,
-  type msg_t <- msg_al_t,
-  type sig_t <- sig_al_t
+clone import DSS_FL.KeyUpdating.EFRMA as DSS_FL_EFRMA with
+  op n_efrma <= qS,
+  op dmsg <= dmsg_fl
   
-  rename [theory] "Stateless" as "AL_SL"
-  rename [theory] "KeyUpdating" as "AL_KU".
-
+  proof *.
+  
+  realize dmsg_ll by exact: dmsg_fl_ll.
+  realize ge0_nefrma by exact: ge0_qS. 
+  
+   
 clone import ROM as MCORO with
   type in_t <- rco_t * msg_al_t,
   type out_t <- msg_fl_t,
@@ -94,7 +102,7 @@ module MCO = ERO.
 clone import Reprogramming as Repro with
     type from <- rco_t * msg_al_t,
     type hash <- msg_fl_t,
-  
+        
       op dhash <- dmsg_fl,
       
   theory MUFF.FinT <= RCOMSGAL,
@@ -104,11 +112,29 @@ clone import Reprogramming as Repro with
   
   proof dhash_ll by exact: dmsg_fl_ll.
 
+clone import EFRMA_Interactive_Equiv as EFRMAEqv with
+  type msg_t <= msg_fl_t,
+  type sig_t <= sig_fl_t,
+  type pk_t <= pk_fl_t,
+  type sk_t <= sk_fl_t,
   
+  op dmsg <= dmsg_fl,
+  op n_efrma <= qS,
+  
+  theory ClassDS <= DSS_FL
+  
+  rename [theory] "Class_EFRMA" as "DSS_FL_EFRMA"
+  
+  proof *.
+
+  realize dmsg_ll by exact: dmsg_fl_ll.
+  realize ge0_nefrma by exact: ge0_qS.
+
+
 (* --- Properties --- *)
 (* -- EF-CMA -- *)
 (* - Oracle Interfaces - *)
-module type Oracle_CMA(S : AL_KU.Scheme) = {
+module type Oracle_CMA(S : DSS_AL.KeyUpdating.Scheme) = {
   proc init(sk_init : sk_al_t) : unit {}
   proc sign(m : msg_al_t) : sig_al_t {S.sign}
   proc fresh(m : msg_al_t) : bool {}
@@ -127,7 +153,7 @@ module type Adv_EFCMA_RO(SO : SOracle_CMA, HO : POracle) = {
 
 
 (* - Oracles - *)
-module (O_CMA : Oracle_CMA) (S : AL_KU.Scheme) = {
+module (O_CMA : Oracle_CMA) (S : DSS_AL.KeyUpdating.Scheme) = {
     var sk : sk_al_t
     var qs : msg_al_t list
     
@@ -166,7 +192,7 @@ module (O_CMA : Oracle_CMA) (S : AL_KU.Scheme) = {
 }.
 
 (* - - *)
-module EF_CMA_RO(S : AL_KU.Scheme, A : Adv_EFCMA_RO, SO : Oracle_CMA, HO : Oracle) = {
+module EF_CMA_RO(S : DSS_AL.KeyUpdating.Scheme, A : Adv_EFCMA_RO, SO : Oracle_CMA, HO : Oracle) = {
   proc main() = {
     var pk : pk_al_t;
     var sk : sk_al_t;
@@ -308,7 +334,7 @@ module M_ETCR_RO(A : Adv_METCR_RO, O : Oracle_METCR, HO : Oracle) = {
 
  
 (* --- Scheme --- *)
-module AL_KU_DSS(FL_KU_DSS : FL_KU.Scheme) : AL_KU.Scheme = {
+module AL_KU_DSS(FL_KU_DSS : DSS_FL.KeyUpdating.Scheme) : DSS_AL.KeyUpdating.Scheme = {
   proc keygen = FL_KU_DSS.keygen
   
   proc sign(sk : sk_al_t, m : msg_al_t) : sig_al_t * sk_al_t = {
@@ -349,7 +375,7 @@ module AL_KU_DSS(FL_KU_DSS : FL_KU.Scheme) : AL_KU.Scheme = {
 
 
 (* --- Reduction Adversaries --- *)
-module (R_EFCMARO_CRRO (FL_KU_DSS : FL_KU.Scheme, A : Adv_EFCMA_RO) : Adv_CR_RO) (HO : POracle) = {
+module (R_EFCMARO_CRRO (FL_KU_DSS : DSS_FL.KeyUpdating.Scheme, A : Adv_EFCMA_RO) : Adv_CR_RO) (HO : POracle) = {
   module O_CMA_R_EFCMARO_CRRO : SOracle_CMA  = {
     var sk : sk_al_t
     var comps : (msg_fl_t * (rco_t * msg_al_t)) list
@@ -403,8 +429,8 @@ module (R_EFCMARO_CRRO (FL_KU_DSS : FL_KU.Scheme, A : Adv_EFCMA_RO) : Adv_CR_RO)
   }
 }.  
 
-search assoc onth. search map zip.
-module (R_EFCMARO_METCRRO (FL_KU_DSS : FL_KU.Scheme, A : Adv_EFCMA_RO) : Adv_METCR_RO) (O : TOracle_METCR, HO : POracle) = {
+
+module (R_EFCMARO_METCRRO (FL_KU_DSS : DSS_FL.KeyUpdating.Scheme, A : Adv_EFCMA_RO) : Adv_METCR_RO) (O : TOracle_METCR, HO : POracle) = {
   module O_CMA_R_EFCMARO_METCRRO : SOracle_CMA  = {
     var sk : sk_al_t
     var comps : (msg_fl_t * (rco_t * msg_al_t)) list
@@ -460,22 +486,175 @@ module (R_EFCMARO_METCRRO (FL_KU_DSS : FL_KU.Scheme, A : Adv_EFCMA_RO) : Adv_MET
 }.  
 
 
+module (R_EFCMARO_IEFRMA(A : Adv_EFCMA_RO) : Adv_I_EFRMA) (O : SOracle_RMA) = {
+  module O_CMA_R_EFCMARO_IEFRMA : SOracle_CMA = {
+    var qs : msg_al_t list
+    var comps : (msg_fl_t * (rco_t * msg_al_t)) list 
+    
+    proc init() = {
+      qs <- [];
+      comps <- [];
+    }
+    
+    proc sign(m : msg_al_t) : sig_al_t = {
+      var rco : rco_t;
+      var cm : msg_fl_t;
+      var sigfl : sig_fl_t;
+      var sig : sig_al_t;
+
+      rco <$ drco;
+
+      (cm, sigfl) <@ O.sign();
+     
+      Wrapped_Oracle(MCO).set((rco, m), cm);
+      
+      cm <@ Wrapped_Oracle(MCO).o((rco, m));
+
+      sig <- (rco, sigfl);
+      
+      comps <- rcons comps (cm, (rco, m));
+      qs <- rcons qs m;
+      
+      return sig;
+    }
+  }
+  
+  proc forge(pk : pk_fl_t) : msg_fl_t * sig_fl_t = {
+    var m : msg_al_t;
+    var sig : sig_al_t;
+    var rco : rco_t;
+    var cm : msg_fl_t;
+    var sigfl : sig_fl_t;
+        
+    MCO.init();
+    Wrapped_Oracle(MCO).init();
+    O_CMA_R_EFCMARO_IEFRMA.init();
+    
+    (m, sig) <@ A(O_CMA_R_EFCMARO_IEFRMA, Wrapped_Oracle(MCO)).forge(pk); 
+    
+    rco <- sig.`1;
+    sigfl <- sig.`2;
+    
+    cm <@ Wrapped_Oracle(MCO).o((rco, m));
+    
+    return (cm, sigfl);
+  }
+}.
+(*
+module QC_RO (O : POracle) : POracle = {
+  var cH : int
+  
+  proc o(x : rco_t * msg_al_t) : msg_fl_t = {
+    var cm : msg_fl_t;
+    
+    cH <- cH + 1;
+    
+    cm <@ O.o(x);
+    
+    return cm; 
+  }
+}.
+
+module QC_SO (O : SOracle_CMA) : SOracle_CMA = {
+  var cS : int
+    
+  proc sign(m : msg_al_t) : sig_al_t = {
+    var sig : sig_al_t;
+    
+    cS <- cS + 1;
+    
+    sig <@ O.sign(m);
+    
+    return sig;
+  }
+}.
+
+
+module QC_O (SO : SOracle_CMA) (PO : POracle)  : SOracle_CMA, POracle = {
+  var cS : int
+  var cH : int
+  
+  proc o(x : rco_t * msg_al_t) : msg_fl_t = {
+    var cm : msg_fl_t;
+    
+    cH <- cH + 1;
+    
+    cm <@ PO.o(x);
+    
+    return cm; 
+  }
+  
+  proc sign(m : msg_al_t) : sig_al_t = {
+    var sig : sig_al_t;
+    
+    cS <- cS + 1;
+    
+    sig <@ SO.sign(m);
+    
+    return sig;
+  }
+}.
+*)
+
+
+module (QC_A(A : Adv_EFCMA_RO) : Adv_EFCMA_RO) (SO : SOracle_CMA) (RO : POracle) = {
+  var cS : int
+  var cH : int
+  
+  module QC_SO : SOracle_CMA = {
+    proc sign(m : msg_al_t) : sig_al_t = {
+      var sig : sig_al_t;
+
+      cS <- cS + 1;
+
+      sig <@ SO.sign(m);
+
+      return sig;
+    }
+  }
+  
+  module QC_RO : POracle = {
+    proc o(x : rco_t * msg_al_t) : msg_fl_t = {
+      var cm : msg_fl_t;
+
+      cH <- cH + 1;
+
+      cm <@ RO.o(x);
+
+      return cm; 
+    }
+  }
+  
+  proc forge(pk : pk_al_t) : msg_al_t * sig_al_t = {
+    var m : msg_al_t;
+    var sig : sig_al_t;
+    
+    cS <- 0;
+    cH <- 0;
+    
+    (m, sig) <@ A(QC_SO, QC_RO).forge(pk);
+    
+    return (m, sig); 
+  }
+}.
+
+
 
 section Proof_EFCMA_RO_ALKUDSS.
 
-declare module FL_KU_DSS <: FL_KU.Scheme{-ERO, -O_CMA, -O_METCR, -R_EFCMARO_CRRO, -R_EFCMARO_METCRRO}.
+declare module FL_KU_DSS <: DSS_FL.KeyUpdating.Scheme{-ERO, -O_CMA, -O_METCR, -R_EFCMARO_CRRO, -R_EFCMARO_METCRRO, -Wrapped_Oracle, -RepO, -O_RMA_Default, -R_EFCMARO_IEFRMA, -QC_A}.
 declare axiom FL_KU_DSS_verify_ll : islossless FL_KU_DSS.verify. 
 
-declare module A <: Adv_EFCMA_RO{-FL_KU_DSS, -ERO, -O_CMA, -O_METCR, -R_EFCMARO_CRRO, -R_EFCMARO_METCRRO}.
+declare module A <: Adv_EFCMA_RO{-FL_KU_DSS, -ERO, -O_CMA, -O_METCR, -R_EFCMARO_CRRO, -R_EFCMARO_METCRRO, -Wrapped_Oracle, -RepO, -O_RMA_Default, -R_EFCMARO_IEFRMA, -QC_A}.
 
-(* Signature queries *)
-declare op qS : { int | 0 <= qS } as ge0_qS.
+(*
+declare axiom A_forge_queries (RO <: POracle {-A, -QC_RO, -QC_SO}) (SO <: SOracle_CMA{-A, -QC_RO, -QC_SO}) : 
+  hoare[A(QC_SO(SO), QC_RO(RO)).forge : QC_SO.cS = 0 /\ QC_RO.cH = 0 ==> QC_SO.cS <= qS /\ QC_RO.cH <= qH].
+*)
+declare axiom A_forge_queries (SO <: SOracle_CMA{-A, -QC_A}) (RO <: POracle{-A, -QC_A}):
+  hoare[QC_A(A, SO, RO).forge : true ==> QC_A.cS <= qS /\ QC_A.cH <= qH].
 
-(* Random Oracle (Hash) queries *)
-declare op qH : { int | 0 <= qH } as ge0_qH.  
-
-
-local module O_CMA_Coll = {
+local module O_CMA_CC = {
     var sk : sk_al_t
     var qs : msg_al_t list
     var comps : (msg_fl_t * (rco_t * msg_al_t)) list 
@@ -529,7 +708,7 @@ local module O_CMA_Coll = {
     }
 }.
 
-local module EF_CMA_RO_Coll = {
+local module EF_CMA_RO_CC = {
   var coll : bool
   
   proc main() = {
@@ -549,14 +728,14 @@ local module EF_CMA_RO_Coll = {
     (pk, sk) <@ AL_KU_DSS(FL_KU_DSS).keygen();
 
     (* Initialize the signing oracle with the generated secret key *)
-    O_CMA_Coll.init(sk);
+    O_CMA_CC.init(sk);
 
     (*
       Ask the adversary to forge a signature for any message (and provide both the
       message and the signature) given the public key pk and access to a signing oracle 
       that it can query an unlimited number of times
     *)
-    (m, sig) <@ A(O_CMA_Coll, MCO).forge(pk);
+    (m, sig) <@ A(O_CMA_CC, MCO).forge(pk);
 
     (* 
       Verify (w.r.t. message m) the signature sig provided by the adversary 
@@ -569,12 +748,12 @@ local module EF_CMA_RO_Coll = {
       (i.e., check whether message is not included in the list of messages for which 
       the adversary received signatures through an oracle query)
     *)
-    is_fresh <@ O_CMA_Coll.fresh(m);
+    is_fresh <@ O_CMA_CC.fresh(m);
     
     (* Collision check *)
     rco <- sig.`1;
     cm <@ MCO.o(rco, m);
-    comps <@ O_CMA_Coll.compressions();
+    comps <@ O_CMA_CC.compressions();
     
     coll <- assoc comps cm <> None;
     
@@ -587,41 +766,41 @@ local module EF_CMA_RO_Coll = {
   }
 }.
 
-local equiv Equiv_EFCMARO_EFCMAROColl :
-  EF_CMA_RO(AL_KU_DSS(FL_KU_DSS), A, O_CMA, MCO).main ~ EF_CMA_RO_Coll.main : ={glob FL_KU_DSS, glob A} ==> ={res}.
+local equiv Equiv_EFCMARO_EFCMAROCC :
+  EF_CMA_RO(AL_KU_DSS(FL_KU_DSS), A, O_CMA, MCO).main ~ EF_CMA_RO_CC.main : ={glob FL_KU_DSS, glob A} ==> ={res}.
 proof.
 proc; inline *.
 seq 19 20 : (={is_valid, is_fresh}); last by wp.
-seq 8 9 : (={glob FL_KU_DSS, pk, m, sig, ERO.m} /\ ={qs}(O_CMA, O_CMA_Coll)); last by sim.
-call (: ={glob FL_KU_DSS, ERO.m} /\ ={sk, qs}(O_CMA, O_CMA_Coll)); first by proc.
+seq 8 9 : (={glob FL_KU_DSS, pk, m, sig, ERO.m} /\ ={qs}(O_CMA, O_CMA_CC)); last by sim.
+call (: ={glob FL_KU_DSS, ERO.m} /\ ={sk, qs}(O_CMA, O_CMA_CC)); first by proc.
 + proc; inline{1} 1. 
   by wp; call (: true); call (: ={ERO.m}); auto.
 by wp; call (: true); while (={w, ERO.m}); auto.
 qed.
 
-local lemma EFCMAROColl_CRRO &m:
-  Pr[EF_CMA_RO_Coll.main() @ &m : res /\ EF_CMA_RO_Coll.coll]
+local lemma EFCMAROCC_CRRO &m:
+  Pr[EF_CMA_RO_CC.main() @ &m : res /\ EF_CMA_RO_CC.coll]
   <=
   Pr[CR_RO(R_EFCMARO_CRRO(FL_KU_DSS, A), MCO).main() @ &m : res].
 proof.
 byequiv => //.
 proc; inline{1} 6; inline{2} 2.
-conseq (: _ ==> is_fresh{1} /\ EF_CMA_RO_Coll.coll{1} => kx{2} <> kx'{2} /\ y{2} = y'{2}); 1: by smt().
-seq 4 4 : (   ={sk, comps}(O_CMA_Coll, R_EFCMARO_CRRO.O_CMA_R_EFCMARO_CRRO) 
+conseq (: _ ==> is_fresh{1} /\ EF_CMA_RO_CC.coll{1} => kx{2} <> kx'{2} /\ y{2} = y'{2}); 1: by smt().
+seq 4 4 : (   ={sk, comps}(O_CMA_CC, R_EFCMARO_CRRO.O_CMA_R_EFCMARO_CRRO) 
            /\ (glob MCO){1} = (glob ERO){2}
            /\ m{1} = mal'{2}
            /\ sig{1} = sig'{2}
-           /\ (forall (mfl : msg_fl_t) (rmal : rco_t * msg_al_t), (mfl, rmal) \in O_CMA_Coll.comps{1}
+           /\ (forall (mfl : msg_fl_t) (rmal : rco_t * msg_al_t), (mfl, rmal) \in O_CMA_CC.comps{1}
                  => mfl = oget (MCO.m{1}.[rmal]))
-           /\ (forall (msg : msg_fl_t), assoc O_CMA_Coll.comps{1} msg <> None 
-                 => (oget (assoc O_CMA_Coll.comps{1} msg)).`2 \in O_CMA_Coll.qs{1})).
+           /\ (forall (msg : msg_fl_t), assoc O_CMA_CC.comps{1} msg <> None 
+                 => (oget (assoc O_CMA_CC.comps{1} msg)).`2 \in O_CMA_CC.qs{1})).
 + call (:   ={glob FL_KU_DSS}   
-         /\ ={sk, comps}(O_CMA_Coll, R_EFCMARO_CRRO.O_CMA_R_EFCMARO_CRRO)
+         /\ ={sk, comps}(O_CMA_CC, R_EFCMARO_CRRO.O_CMA_R_EFCMARO_CRRO)
          /\ (glob MCO){1} = (glob ERO){2}
-         /\ (forall (mfl : msg_fl_t) (rmal : rco_t * msg_al_t), (mfl, rmal) \in O_CMA_Coll.comps{1}
+         /\ (forall (mfl : msg_fl_t) (rmal : rco_t * msg_al_t), (mfl, rmal) \in O_CMA_CC.comps{1}
               => mfl = oget (MCO.m{1}.[rmal]))
-         /\ (forall (msg : msg_fl_t), assoc O_CMA_Coll.comps{1} msg <> None
-              => (oget (assoc O_CMA_Coll.comps{1} msg)).`2 \in O_CMA_Coll.qs{1})).
+         /\ (forall (msg : msg_fl_t), assoc O_CMA_CC.comps{1} msg <> None
+              => (oget (assoc O_CMA_CC.comps{1} msg)).`2 \in O_CMA_CC.qs{1})).
   - by proc; skip.
   - proc; inline *.
     wp; call (: true); wp; rnd; skip => /> &1 &2 comps_def compsqs_rel rco _.
@@ -647,31 +826,31 @@ by move=> {3}-> /#.
 qed.
 
 
-local lemma EFCMAROColl_METCRRO &m:
-  Pr[EF_CMA_RO_Coll.main() @ &m : res /\ EF_CMA_RO_Coll.coll]
+local lemma EFCMAROCC_METCRRO &m:
+  Pr[EF_CMA_RO_CC.main() @ &m : res /\ EF_CMA_RO_CC.coll]
   <=
   Pr[M_ETCR_RO(R_EFCMARO_METCRRO(FL_KU_DSS, A), O_METCR, MCO).main() @ &m : res].
 proof.
 byequiv => //.
 proc; inline{2} 3.
-conseq (: _ ==> is_fresh{1} /\ EF_CMA_RO_Coll.coll{1} => 0 <= i{2} < nrts{2} /\ x{2} <> x'{2} /\ y{2} = y'{2}); 1: by smt().
-seq 4 5 : (   ={sk, comps}(O_CMA_Coll, R_EFCMARO_METCRRO.O_CMA_R_EFCMARO_METCRRO) 
+conseq (: _ ==> is_fresh{1} /\ EF_CMA_RO_CC.coll{1} => 0 <= i{2} < nrts{2} /\ x{2} <> x'{2} /\ y{2} = y'{2}); 1: by smt().
+seq 4 5 : (   ={sk, comps}(O_CMA_CC, R_EFCMARO_METCRRO.O_CMA_R_EFCMARO_METCRRO) 
            /\ (glob MCO){1} = (glob ERO){2}
            /\ m{1} = mal'{2}
            /\ sig{1} = sig'{2}
            /\ unzip2 R_EFCMARO_METCRRO.O_CMA_R_EFCMARO_METCRRO.comps{2} = O_METCR.ts{2}
-           /\ (forall (mfl : msg_fl_t) (rmal : rco_t * msg_al_t), (mfl, rmal) \in O_CMA_Coll.comps{1}
+           /\ (forall (mfl : msg_fl_t) (rmal : rco_t * msg_al_t), (mfl, rmal) \in O_CMA_CC.comps{1}
                  => mfl = oget (MCO.m{1}.[rmal]))
-           /\ (forall (msg : msg_fl_t), assoc O_CMA_Coll.comps{1} msg <> None 
-                 => (oget (assoc O_CMA_Coll.comps{1} msg)).`2 \in O_CMA_Coll.qs{1})).
+           /\ (forall (msg : msg_fl_t), assoc O_CMA_CC.comps{1} msg <> None 
+                 => (oget (assoc O_CMA_CC.comps{1} msg)).`2 \in O_CMA_CC.qs{1})).
 + call (:   ={glob FL_KU_DSS}   
-         /\ ={sk, comps}(O_CMA_Coll, R_EFCMARO_METCRRO.O_CMA_R_EFCMARO_METCRRO)
+         /\ ={sk, comps}(O_CMA_CC, R_EFCMARO_METCRRO.O_CMA_R_EFCMARO_METCRRO)
          /\ (glob MCO){1} = (glob ERO){2}
          /\ unzip2 R_EFCMARO_METCRRO.O_CMA_R_EFCMARO_METCRRO.comps{2} = O_METCR.ts{2}
-         /\ (forall (mfl : msg_fl_t) (rmal : rco_t * msg_al_t), (mfl, rmal) \in O_CMA_Coll.comps{1}
+         /\ (forall (mfl : msg_fl_t) (rmal : rco_t * msg_al_t), (mfl, rmal) \in O_CMA_CC.comps{1}
               => mfl = oget (MCO.m{1}.[rmal]))
-         /\ (forall (msg : msg_fl_t), assoc O_CMA_Coll.comps{1} msg <> None
-              => (oget (assoc O_CMA_Coll.comps{1} msg)).`2 \in O_CMA_Coll.qs{1})).
+         /\ (forall (msg : msg_fl_t), assoc O_CMA_CC.comps{1} msg <> None
+              => (oget (assoc O_CMA_CC.comps{1} msg)).`2 \in O_CMA_CC.qs{1})).
   - by proc; skip.
   - proc; inline *.
     wp; call (: true); wp; rnd; wp; skip => /> &1 &2 comps_def compsqs_rel rco _.
@@ -704,4 +883,481 @@ rewrite eq_sym -{1}(zip_unzip R_EFCMARO_METCRRO.O_CMA_R_EFCMARO_METCRRO.comps{2}
 by rewrite assoc_zip 1:2!size_map // nth_onth /oget /#.
 qed.
 
+local module O_CMA_CC_NoRepro = {
+  include var O_CMA_CC [-sign]
+
+  (* 
+    Sign given message m using the considered signature scheme with the
+    secret/signing key sk and append m to the list of oracle queries qs
+  *)
+  proc sign(m : msg_al_t) : sig_al_t = {
+    var rco : rco_t;
+    var cm : msg_fl_t;
+    var sigfl : sig_fl_t;
+    var sig : sig_al_t;
+
+    rco <$ drco;
+    cm <$ dmsg_fl;
+    
+    cm <@ Wrapped_Oracle(MCO).o((rco, m));
+
+    (sigfl, sk) <@ FL_KU_DSS.sign(sk, cm);
+
+    sig <- (rco, sigfl);
+
+    comps <- rcons comps (cm, (rco, m));
+    qs <- rcons qs m;
+
+    return sig;
+  }
+}.
+
+
+local module EF_CMA_RO_CC_NoRepro = {
+  var coll : bool
+  
+  proc main() = {
+    var pk : pk_al_t;
+    var sk : sk_al_t;
+    var m : msg_al_t;
+    var sig : sig_al_t;
+    var is_valid, is_fresh : bool;
+    var rco : rco_t;
+    var cm : msg_fl_t;
+    var comps : (msg_fl_t * (rco_t * msg_al_t)) list;
+    
+    (* Initialize (hash) random oracle *)
+    MCO.init();
+    Wrapped_Oracle(MCO).init();
+    
+    (* Generate a key pair using the considered signature scheme *)
+    (pk, sk) <@ AL_KU_DSS(FL_KU_DSS).keygen();
+
+    (* Initialize the signing oracle with the generated secret key *)
+    O_CMA_CC_NoRepro.init(sk);
+
+    (*
+      Ask the adversary to forge a signature for any message (and provide both the
+      message and the signature) given the public key pk and access to a signing oracle 
+      that it can query an unlimited number of times
+    *)
+    (m, sig) <@ A(O_CMA_CC_NoRepro, Wrapped_Oracle(MCO)).forge(pk);
+
+    (* 
+      Verify (w.r.t. message m) the signature sig provided by the adversary 
+      using the verification algorithm of the considered signature scheme 
+    *)
+    is_valid <@ AL_KU_DSS(FL_KU_DSS).verify(pk, m, sig);
+
+    (* 
+      Check whether message for which the adversary forged a signature is fresh 
+      (i.e., check whether message is not included in the list of messages for which 
+      the adversary received signatures through an oracle query)
+    *)
+    is_fresh <@ O_CMA_CC_NoRepro.fresh(m);
+    
+    (* Collision check *)
+    rco <- sig.`1;
+    cm <@ Wrapped_Oracle(MCO).o(rco, m);
+    comps <@ O_CMA_CC_NoRepro.compressions();
+    
+    coll <- assoc comps cm <> None;
+    
+    (* 
+      Success iff
+      (1) "is_valid": the forged signature provided by the adversary is valid, and
+      (2) "is_fresh": the message for which the adversary forged a signature is fresh.
+    *)
+    return is_valid /\ is_fresh;
+  }
+}.
+
+
+local equiv Equiv_EFCMAROCC_EFCMAROCCNRepro :
+  EF_CMA_RO_CC.main ~ EF_CMA_RO_CC_NoRepro.main : ={glob FL_KU_DSS, glob A} ==> ={res}.
+proof.
+proc. inline *. wp => /=.
+call (: true).
+wp.
+call (: ={glob O_CMA_CC, glob MCO} /\ Wrapped_Oracle.prog_list{2} = []).
+proc. inline *. wp. skip. by progress.
+proc. inline *. wp. call (: true). wp. rnd{2}. rnd. skip. progress.
+wp.
+call (: true).
+wp. 
+while (={w, ERO.m}).
+sim.
+wp.
+by skip.
+qed.
+  
+local module O_CMA_CC_ReproSample = {
+  include var O_CMA_CC [-sign]
+
+  (* 
+    Sign given message m using the considered signature scheme with the
+    secret/signing key sk and append m to the list of oracle queries qs
+  *)
+  proc sign(m : msg_al_t) : sig_al_t = {
+    var rco : rco_t;
+    var cm : msg_fl_t;
+    var sigfl : sig_fl_t;
+    var sig : sig_al_t;
+
+    rco <$ drco;
+    cm <$ dmsg_fl;
+    
+    Wrapped_Oracle(MCO).set((rco, m), cm);
+    cm <@ Wrapped_Oracle(MCO).o((rco, m));
+
+    (sigfl, sk) <@ FL_KU_DSS.sign(sk, cm);
+
+    sig <- (rco, sigfl);
+
+    comps <- rcons comps (cm, (rco, m));
+    qs <- rcons qs m;
+
+    return sig;
+  }
+}.
+
+
+local module EF_CMA_RO_CC_ReproSample = {
+  var coll : bool
+  
+  proc main() = {
+    var pk : pk_al_t;
+    var sk : sk_al_t;
+    var m : msg_al_t;
+    var sig : sig_al_t;
+    var is_valid, is_fresh : bool;
+    var rco : rco_t;
+    var cm : msg_fl_t;
+    var comps : (msg_fl_t * (rco_t * msg_al_t)) list;
+    
+    (* Initialize (hash) random oracle *)
+    MCO.init();
+    Wrapped_Oracle(MCO).init();
+    
+    (* Generate a key pair using the considered signature scheme *)
+    (pk, sk) <@ AL_KU_DSS(FL_KU_DSS).keygen();
+
+    (* Initialize the signing oracle with the generated secret key *)
+    O_CMA_CC_ReproSample.init(sk);
+
+    (*
+      Ask the adversary to forge a signature for any message (and provide both the
+      message and the signature) given the public key pk and access to a signing oracle 
+      that it can query an unlimited number of times
+    *)
+    (m, sig) <@ A(O_CMA_CC_ReproSample, Wrapped_Oracle(MCO)).forge(pk);
+
+    (* 
+      Verify (w.r.t. message m) the signature sig provided by the adversary 
+      using the verification algorithm of the considered signature scheme 
+    *)
+    is_valid <@ AL_KU_DSS(FL_KU_DSS).verify(pk, m, sig);
+
+    (* 
+      Check whether message for which the adversary forged a signature is fresh 
+      (i.e., check whether message is not included in the list of messages for which 
+      the adversary received signatures through an oracle query)
+    *)
+    is_fresh <@ O_CMA_CC_ReproSample.fresh(m);
+    
+    (* Collision check *)
+    rco <- sig.`1;
+    cm <@ Wrapped_Oracle(MCO).o(rco, m);
+    comps <@ O_CMA_CC_ReproSample.compressions();
+    
+    coll <- assoc comps cm <> None;
+    
+    (* 
+      Success iff
+      (1) "is_valid": the forged signature provided by the adversary is valid, and
+      (2) "is_fresh": the message for which the adversary forged a signature is fresh.
+    *)
+    return is_valid /\ is_fresh;
+  }
+}.
+
+local module (R_Repro_EFCMARORepro : DistA) (WMCO : POracle, RepWMCO : RepO_t) = {
+  module O_R_Repro_EFCMARORepro = {
+    include var O_CMA_CC [-sign]
+    
+    proc sign(m : msg_al_t) : sig_al_t = {
+      var rco : rco_t;
+      var cm : msg_fl_t;
+      var sigfl : sig_fl_t;
+      var sig : sig_al_t;
+      
+      (rco, m) <@ RepWMCO.repro(dmap drco (fun (rco : rco_t) => (rco, m)));
+      
+      cm <@ WMCO.o((rco, m));
+      
+      (sigfl, sk) <@ FL_KU_DSS.sign(sk, cm);
+      
+      sig <- (rco, sigfl);
+      
+      comps <- rcons comps (cm, (rco, m));
+      qs <- rcons qs m;
+      
+      return sig;
+    } 
+  }
+  
+  proc distinguish() : bool = {
+    var pk : pk_al_t;
+    var sk : sk_al_t;
+    var m : msg_al_t;
+    var sig : sig_al_t;
+    var is_valid, is_fresh : bool;
+    var rco : rco_t;
+    var cm : msg_fl_t;
+    var comps : (msg_fl_t * (rco_t * msg_al_t)) list;
+    var coll : bool;
+    
+    (pk, sk) <@ AL_KU_DSS(FL_KU_DSS).keygen();
+    
+    O_R_Repro_EFCMARORepro.init(sk);
+    
+    (m, sig) <@ A(O_R_Repro_EFCMARORepro, WMCO).forge(pk);
+    
+    is_valid <@ AL_KU_DSS(FL_KU_DSS).verify(pk, m, sig);
+
+    is_fresh <@ O_R_Repro_EFCMARORepro.fresh(m);
+    
+    rco <- sig.`1;
+    cm <@ WMCO.o(rco, m);
+    comps <@ O_R_Repro_EFCMARORepro.compressions();
+    
+    coll <- assoc comps cm <> None;
+
+    return is_valid /\ is_fresh /\ !coll;
+  }
+}.
+
+local lemma EFCMARORepro_ReproGame &m:
+  `| Pr[EF_CMA_RO_CC_NoRepro.main() @ &m : res /\ !EF_CMA_RO_CC_NoRepro.coll] -
+     Pr[EF_CMA_RO_CC_ReproSample.main() @ &m : res /\ !EF_CMA_RO_CC_ReproSample.coll] |
+  =
+  `| Pr[ReproGame(MCO, R_Repro_EFCMARORepro).main(false) @ &m : res] -
+     Pr[ReproGame(MCO, R_Repro_EFCMARORepro).main(true) @ &m : res] |.
+proof.
+do 2! congr; last congr.
++ byequiv => //.
+  proc; inline *.
+  wp; call (: true); wp => /=.
+  call (:   ={glob FL_KU_DSS, glob O_CMA_CC, Wrapped_Oracle.prog_list} 
+         /\ RepO.b{2} = false
+         /\ Wrapped_Oracle.prog_list{2} = []).
+  - proc; inline *. 
+    by wp; skip.
+  - proc; inline *.
+    rcondf{2} 5; 1: by auto.
+    wp; call (: true); wp => /=.
+    rnd{1}.
+    rnd (fun (rco : rco_t) => (rco, m{2})) 
+        (fun (kx : rco_t * msg_al_t) => kx.`1).
+    wp; skip => /> &1.
+    split => [rcom | rcomeq].
+    * by move/supp_dmap => [rco] [_ ->].
+    split => [rcom rcomin | rcom_mu1 rco rcoin].
+    * by rewrite (in_dmap1E_can _ _ (fun (x : _ * _) => x.`1)) //= /#.
+    by rewrite supp_dmap; exists rco; rewrite rcoin.
+  wp; call (: true); wp; while (={w, ERO.m}).
+  - by wp; rnd; wp; skip.
+  by wp; skip.
+byequiv => //.
+proc; inline *.
+wp; call (: true); wp => /=.
+call (:   ={glob FL_KU_DSS, glob O_CMA_CC, Wrapped_Oracle.prog_list} 
+       /\ RepO.b{2} = true).
++ proc; inline *. 
+  by wp; skip.
++ proc; inline *.
+  rcondt{2} 5; 1: by auto.
+  wp; call (: true); wp => /=.
+  rnd.
+  rnd (fun (rco : rco_t) => (rco, m{2})) 
+      (fun (kx : rco_t * msg_al_t) => kx.`1).
+  wp; skip => /> &1.
+  split => [rcom | rcomeq].
+  * by move/supp_dmap => [rco] [_ ->].
+  split => [rcom rcomin | rcom_mu1 rco rcoin].
+  * by rewrite (in_dmap1E_can _ _ (fun (x : _ * _) => x.`1)) //= /#.
+  by rewrite supp_dmap; exists rco; rewrite rcoin.
+wp; call (: true); wp; while (={w, ERO.m}).
++ by wp; rnd; wp; skip.
+by wp; skip.
+qed.
+
+
+local module O_CMA_CC_ReproQuery = {
+  include var O_CMA_CC [-init, sign]
+
+  proc init() = {
+    qs <- [];
+    comps <- [];
+  }
+
+  proc sign(m : msg_al_t) : sig_al_t = {
+    var rco : rco_t;
+    var cm : msg_fl_t;
+    var sigfl : sig_fl_t;
+    var sig : sig_al_t;
+
+    rco <$ drco;
+    
+    (cm, sigfl) <@ O_RMA_Default(FL_KU_DSS).sign();
+
+    Wrapped_Oracle(MCO).set((rco, m), cm);
+    cm <@ Wrapped_Oracle(MCO).o((rco, m));
+
+    sig <- (rco, sigfl);
+
+    comps <- rcons comps (cm, (rco, m));
+    qs <- rcons qs m;
+
+    return sig;
+  }
+}.
+
+
+local module EF_CMA_RO_CC_ReproQuery = {
+  var coll : bool
+  
+  proc main() = {
+    var pk : pk_al_t;
+    var sk : sk_al_t;
+    var m : msg_al_t;
+    var sig : sig_al_t;
+    var is_valid, is_fresh : bool;
+    var rco : rco_t;
+    var cm : msg_fl_t;
+    var comps : (msg_fl_t * (rco_t * msg_al_t)) list;
+    var nrqs : int;
+    
+    (* Initialize (hash) random oracle *)
+    MCO.init();
+    Wrapped_Oracle(MCO).init();
+    
+    (* Generate a key pair using the considered signature scheme *)
+    (pk, sk) <@ AL_KU_DSS(FL_KU_DSS).keygen();
+
+    (* Initialize the signing oracle with the generated secret key *)
+    O_RMA_Default(FL_KU_DSS).init(sk);
+    O_CMA_CC_ReproQuery.init();
+
+    (*
+      Ask the adversary to forge a signature for any message (and provide both the
+      message and the signature) given the public key pk and access to a signing oracle 
+      that it can query an unlimited number of times
+    *)
+    (m, sig) <@ QC_A(A, O_CMA_CC_ReproQuery, Wrapped_Oracle(MCO)).forge(pk);
+
+    (* 
+      Verify (w.r.t. message m) the signature sig provided by the adversary 
+      using the verification algorithm of the considered signature scheme 
+    *)
+    is_valid <@ AL_KU_DSS(FL_KU_DSS).verify(pk, m, sig);
+
+    (* 
+      Check whether message for which the adversary forged a signature is fresh 
+      (i.e., check whether message is not included in the list of messages for which 
+      the adversary received signatures through an oracle query)
+    *)
+    is_fresh <@ O_CMA_CC_ReproQuery.fresh(m);
+    
+    (* Collision check *)
+    rco <- sig.`1;
+    cm <@ Wrapped_Oracle(MCO).o(rco, m);
+    comps <@ O_CMA_CC_ReproSample.compressions();
+    
+    coll <- assoc comps cm <> None;
+    
+    (* Get number of signing queries *)
+    nrqs <@ O_CMA_CC_ReproQuery.nr_queries();
+    
+    (* 
+      Success iff
+      (1) "is_valid": the forged signature provided by the adversary is valid, and
+      (2) "is_fresh": the message for which the adversary forged a signature is fresh.
+    *)
+    return nrqs <= qS /\ is_valid /\ is_fresh;
+  }
+}.
+
+local lemma EFRMAROCCReproSample_Query &m:
+  Pr[EF_CMA_RO_CC_ReproSample.main() @ &m : res /\ !EF_CMA_RO_CC_ReproSample.coll]
+  =
+  Pr[EF_CMA_RO_CC_ReproQuery.main() @ &m : res /\ !EF_CMA_RO_CC_ReproQuery.coll].
+proof.
+byequiv => //.
+proc.
+seq 5 6 : (   ={glob FL_KU_DSS, O_CMA_CC.comps, O_CMA_CC.qs, MCO.m, Wrapped_Oracle.prog_list, pk, m, sig}
+           /\ QC_A.cS{2} = size O_CMA_CC.qs{2}
+           /\ QC_A.cS{2} <= qS).
++ call (:   ={glob FL_KU_DSS, glob A, O_CMA_CC.comps, O_CMA_CC.qs, MCO.m, Wrapped_Oracle.prog_list, pk} 
+         /\ ={sk}(O_CMA_CC, O_RMA_Default)
+         /\ O_CMA_CC.qs{2} = []
+           ==> 
+            ={res, glob FL_KU_DSS, O_CMA_CC.comps, O_CMA_CC.qs, MCO.m, Wrapped_Oracle.prog_list}
+         /\ ={sk}(O_CMA_CC, O_RMA_Default)
+         /\ QC_A.cS{2} = size O_CMA_CC.qs{2}
+         /\ QC_A.cS{2} <= qS).
+  - conseq (:   ={arg, glob FL_KU_DSS, glob A, O_CMA_CC.comps, O_CMA_CC.qs, MCO.m, Wrapped_Oracle.prog_list} 
+             /\ ={sk}(O_CMA_CC, O_RMA_Default)
+             /\ O_CMA_CC.qs{2} = []
+               ==> 
+                ={res, glob FL_KU_DSS, O_CMA_CC.comps, O_CMA_CC.qs, MCO.m, Wrapped_Oracle.prog_list} 
+             /\ ={sk}(O_CMA_CC, O_RMA_Default)
+             /\ QC_A.cS{2} = size O_CMA_CC.qs{2})
+           _
+           (: true ==> QC_A.cS <= qS /\ QC_A.cH <= qH) => //.
+    * by apply (A_forge_queries O_CMA_CC_ReproQuery (Wrapped_Oracle(MCO))).
+    proc *; inline *.
+    wp.
+    call (:   ={glob FL_KU_DSS, O_CMA_CC.comps, O_CMA_CC.qs, MCO.m, Wrapped_Oracle.prog_list}
+           /\ ={sk}(O_CMA_CC, O_RMA_Default)
+           /\ QC_A.cS{2} = size O_CMA_CC.qs{2}).
+    * proc; inline *.
+      by wp; skip.
+    * proc; inline *.
+      wp; call (: true); wp => /=.
+      rnd; rnd.
+      by wp; skip => />; smt(size_rcons).
+    by wp; skip => /> /#.
+  inline *.
+  wp; call (: true); wp => /=. 
+  while (={w, ERO.m}); 1: by auto.
+  by wp; skip.
+inline *.
+wp; call(: true); wp => /=.  
+by skip => />. 
+qed.
+
+local lemma EFRMAROCCReproQuery_IEFRMA &m :
+  Pr[EF_CMA_RO_CC_ReproQuery.main() @ &m : res /\ !EF_CMA_RO_CC_ReproQuery.coll]
+  =
+  Pr[I_EF_RMA(FL_KU_DSS, R_EFCMARO_IEFRMA(A), O_RMA_Default).main() @ &m : res].
+proof.
+byequiv => //.
+proc; inline *.
+wp; call (: true); wp => /=.
+call (:    ={glob FL_KU_DSS, MCO.m, Wrapped_Oracle.prog_list, O_RMA_Default.sk}
+        /\ ={qs, comps}(O_CMA_CC, R_EFCMARO_IEFRMA.O_CMA_R_EFCMARO_IEFRMA)).
++ admit.
++ admit.
+swap{1} 6 -5; wp.
+while (={w, ERO.m}); 1: by auto.
+wp; call(:true); wp => /=.
+skip => />.
+progress.
+admit. admit. admit.
+admit.
+admit.
+admit.
+qed.
+  
 end section Proof_EFCMA_RO_ALKUDSS.
